mvcgen 은 아직 시험판이라...하지만 stateful 한 프로그램에는, 필수적인 기능 아닌가.

src/lean/Nemonuri/Study/StanfordOnline/Compilers/Introduction/Basic.lean
@@ -1,6 +1,9 @@
 module
 
-public section
+public import Std.Tactic.Do
+
+public section public_s
+@[expose] section expose_s
 
 namespace Nemonuri.Study.StanfordOnline.Compilers.Introduction
 
@@ -30,34 +33,164 @@ So, what does an interpreter do?
 
 1. You wrote a **Program**(*prog*).
 2. You have a **Data**(*data*), whatever you want to run the program on.
-3. An **Interpreter**(*self*) takes as input, your program(*prog*) and your data(*data*).
-4. It(*self*) produces the output directly.
-5. Meaning that it(*self*) doesn't do any processing of the program(*prog*) before it executes it on the input.
-6. So you just write the program(*prog*), and you invoke the interpreter(*self*) on the data(*data*), and the program(*prog*) immediately begins running.
+3. An **Interpreter**(*s*) takes as input, your program(*prog*) and your data(*data*).
+4. It(*s*) produces the **Output**(*output*) directly.
+5. Meaning that it(*s*) *doesn't do any processing* of the program(*prog*) before it executes it on the input.
+6. So you just write the program(*prog*), and you invoke the interpreter(*s*) on the data(*data*), and the program(*prog*) immediately begins running.
 
 -/
 
+section interpreter_s
 
-structure ProgramCode (α: Type u) where
-  val : α
+universe u1 u2 u3
+variable {TProgram: Type u1} {TData: Type u2} {TOutput: Type u3}
 
-
-structure Data (α: Type u) where
-  val : α
-
-
-inductive ProcessedState where
-  | pre
-  | post
-
-deriving instance DecidableEq, Hashable, Repr, BEq, ReflBEq, LawfulBEq
-  for ImplementationApproach, ProgramCode, Data, ProcessedState
+namespace Interpreter
 
 
+inductive Index where
+  | init
+  | takeInput
+  | produceOutput
+  deriving DecidableEq, Hashable, BEq, ReflBEq, LawfulBEq
+
+instance instInhabitedIndex : Inhabited Index where default := Index.init
+
+
+inductive IndexedState (TProgram: Type u1) (TData: Type u2) (TOutput: Type u3) : Index → Type _ where
+  | init : IndexedState TProgram TData TOutput Index.init
+  | takeInput
+    (pre: IndexedState TProgram TData TOutput Index.init)
+    (prog: TProgram) (data: TData)
+    : IndexedState TProgram TData TOutput Index.takeInput
+  | produceOutput
+    (pre: IndexedState TProgram TData TOutput Index.takeInput)
+    (prog: TProgram)
+    (output: TOutput)
+    : IndexedState TProgram TData TOutput Index.produceOutput
+
+instance instInhabitedIndexedState : Inhabited (IndexedState TProgram TData TOutput (Inhabited.default)) where
+  default := .init
+
+
+
+def invTakeInput
+  (state: IndexedState TProgram TData TOutput Index.takeInput)
+  :=
+  match state with
+  | .takeInput pre prog data => (pre, prog, data)
+
+
+def invProduceOutput
+  (state: IndexedState TProgram TData TOutput Index.produceOutput)
+  :=
+  match state with
+  | .produceOutput pre prog output => (pre, prog, output)
+
+
+structure State (TProgram: Type u1) (TData: Type u2) (TOutput: Type u3) where
+  index: Index
+  indexed: IndexedState TProgram TData TOutput index
+
+instance instInhabitedState : Inhabited (State TProgram TData TOutput) where
+  default := State.mk (Inhabited.default) (Inhabited.default)
+
+namespace Predicates
+
+
+def doesn't_do_any_processing (state: State TProgram TData TOutput) : Prop :=
+  if index_eq : state.index = Index.produceOutput then
+    match (index_eq ▸ state.indexed) |> invProduceOutput with
+    | (pre, postProg, _) =>
+    match invTakeInput pre with
+    | (_, preProg, _) => preProg = postProg
+  else
+    True
+
+
+end Predicates
+
+
+structure LawfulState (TProgram: Type u1) (TData: Type u2) (TOutput: Type u3) where
+  state: State TProgram TData TOutput
+  doesn't_do_any_processing: Predicates.doesn't_do_any_processing state
+
+instance instInhabitedLawfulState : Inhabited (LawfulState TProgram TData TOutput) where
+  default := LawfulState.mk (Inhabited.default) (by unfold Predicates.doesn't_do_any_processing; trivial)
+
+end Interpreter
+
+
+structure Interpreter (TProgram: Type u1) (TData: Type u2) (TOutput: Type u3) where
+  execute:
+    {pre: Interpreter.LawfulState TProgram TData TOutput // pre.state.index = .takeInput} →
+    {post: Interpreter.LawfulState TProgram TData TOutput // post.state.index = .produceOutput}
+  state: Interpreter.LawfulState TProgram TData TOutput
+
+@[reducible]
+def index (x: Interpreter TProgram TData TOutput) : Interpreter.Index :=
+  x.state.state.index
+
+
+@[reducible]
+def InterpreterM (TProgram: Type u1) (TData: Type u2) (TOutput: Type u3) :=
+  StateM (Interpreter TProgram TData TOutput)
+
+
+namespace InterpreterM
+
+open Std.Do
+open Interpreter
+
+def init : (InterpreterM TProgram TData TOutput) PUnit := modify (fun s => { s with state := default })
+
+
+@[spec]
+theorem init_spec :
+  ⦃fun (_: Interpreter TProgram TData TOutput) => ⌜True⌝⦄
+  init
+  ⦃⇓ _ s => ⌜index s = Index.init⌝⦄
+  := by
+  mvcgen [init] with grind
+
+#print init_spec
+
+/-
+def invoke (prog: TProgram) (data: TData) : (InterpreterM TProgram TData TOutput) (ULift TOutput) := do
+  ← init ()
+  ← modify (fun self => Interpreter.IndexedState.takeInput self prog data |> )
+-/
+
+
+
+end InterpreterM
+
+
+
+end interpreter_s
 
 
 
 
+/-
+
+inductive Interpreter (TProgram: Type u1) (TData: Type u2) (TOutput: Type u3) : Interpreter.Index → Type (max u1 u2) where
+  | takeInput (prog: TProgram) (data: TData) : Interpreter TProgram TData TOutput Interpreter.Index.takeInput
+  | produceOutput
+    (preIndex: {x: Interpreter.Index // x = .takeInput})
+    (pre: Interpreter TProgram TData TOutput preIndex.val)
+    (output: TOutput)
+-/
+
+
+/-
+@[expose]
+abbrev anyProcessingInvoked (pre: TProgram) (post: TProgram) := pre ≠ post
+
+structure Interpreter (TData: Type u2) (TOutput: Type u3) where
+  beforeExecute : (pre: TProgram) → { post: TProgram // Not (anyProcessingInvoked pre post) }
+  execute : (prog: TProgram) → (data: TData) → { r: TProgram × TOutput // Not (anyProcessingInvoked r.fst prog) }
+-/
 
 
 /-
@@ -81,6 +214,5 @@ instance instDecidableProcessed {p: Prop} [dp: Decidable p] : Decidable (Process
 
 end Nemonuri.Study.StanfordOnline.Compilers.Introduction
 
-
-
-end --public
+end expose_s
+end public_s
